\begin{equation}
    \begin{array}{lll}
\th_3(0|{2\tau\over 3})~\th_3(\tau|6\tau) &-\th_2(0|{2\tau\over
  3})~\th_2(\tau|6\tau) &= q^{-1/12}~\eta^2 \\
\th_3(0|{3\tau\over 2})~\th_3({1\over 3}|{\tau\over 6})
 & -\th_4(0|{3\tau\over 2})~\th_4({1\over 3}|{\tau\over 6}) &= 2\eta^2 \\  
\th_3(0|6\tau)~\th_2({2\over 3}|{2\tau\over 3})
 &+ \th_3(0|6\tau)~\th_3({2\over 3}|{2\tau\over 3})&= \eta^2 \\ 
\th_4(0|{\tau\over 6})~\th_3(\tau|{3\tau\over 2})
&-\th_3(0|{\tau\over 6})~\th_4(\tau|{3\tau\over 2}) &=q^{-1/3}~\eta^2. 
    \end{array}
  \end{equation}

