\begin{equation*}
  \begin{array}{rl}
A &= {1\over 2\eta^2}\Big[ \th_2(0|6\tau) (\theta_{-12} +
 \theta_{12}) + \th_3(0|6\tau) (\theta_{0} + \theta_{24}) + 
  \th_4(0|2\tau) (\theta_{0} -\theta_{24})\Big]\\ 
  &= {1\over 2\eta^2}\Big[ \th_2(0|6\tau)
 (-q^{1/4})\th_3(2\tau|6\tau)
 +\th_3(0|6\tau)~\th_3(\tau|6\tau)
 +\underbrace{\th_4(0|2\tau)~\th_4(\tau|6\tau)}_{q^{-1/12}~\eta^2} \Big] = q^{-1/12} \\
B &= C= D = E = 0\\
F &= e^{-2\pi i/3} ~q^{-1/12}\\
G &= {q^{1/12}\over \eta^2} \th_3(\tau|6\tau) ~(\theta_{-20} +
 \theta_{4}) + {q^{1/3}\over \eta^2} \th_3(2\tau|6\tau) ~(\theta_{-8} +
 \theta_{16}) = 0 \\
H &= 0 \\
I &=  e^{-2\pi i/6} ~q^{-1/12}\\
  \end{array}
\end{equation*}

