\begin{equation}
\label{S-transf}
\begin{array}{c}
\left(\begin{array}{l} C_{(2)} \\ B \end{array}\right) \to
\left(\begin{array}{cc} r & -s \\ -t & u \end{array}\right)
\left(\begin{array}{l} C_{(2)} \\ B \end{array}\right)\;;\;
\left(\begin{array}{l} \tilde{F} \\ F \end{array}\right) \to
\left(\begin{array}{cc} r & s \\ t & u \end{array}\right)
\left(\begin{array}{l} \tilde{F} \\ F \end{array}\right)\;;
\\ \\
\displaystyle \tau \to \frac{r\tau+s}{t\tau+u}\,,
\text{ where } \tau = \C + ie^{-\Phi}.
\end{array}
\end{equation}

