\begin{equation}
\begin{align}
{}& \text{(i) Functional equation:} \quad
e_b(x-i\fr{b}{2})=(1+e^{2\pi bx})e_b(x+i\fr{b}{2}). \label{e_feq}\\
{}& \text{(ii) Unitarity:}\qquad
|e_b(x)|=1\quad\text{for $x\in\BR$}. \label{e_unit}\\
{}& \text{(iii) Analyticity:}\quad
s_b(x)\;\text{is meromorphic,}\nonumber\\ 
{}& \hspace{2.7cm}\text{poles:}\;\,  
x=c_b+i(nb+mb^{-1}), n,m\in\BZ^{\geq 0}.\\
{}& \hspace{2.7cm}\text{zeros:}\;\,  
x=-c_b-i(nb+mb^{-1}), n,m\in\BZ^{\geq 0}.\nonumber 
%{}& \text{(iii) Inversion relation:}\qquad 
%e_b(x)e_b(-x)=e^{\pi i x^2}e^{-\frac{\pi i}{12}(2-Q^2)}.
\end{align}
% \end{equation}

