\begin{equation}  \label{t6}
  \begin{array}{ll}
\th_1(v|\tau)= -i \sum_{n\in\Z} (-1)^n q^{(n+\half)^2/2} y^{n+\half} 
   &= 2q^{1\over 8}\sin[\pi v]\prod_{n=1}^{\infty}
   (1-q^n)(1-q^n y)(1-q^n y^{-1})\\
\th_2(v|\tau)=\sum q^{(n+\half)^2/2} y^{n+\half}
&=2q^{1\over 8}\cos[\pi v]\prod (1-q^n)(1+q^n y)(1+q^n y^{-1})\\
\th_3(v|\tau)= \sum q^{n^2/2} y^n
&=\prod (1-q^n)(1+q^{n-1/2} y)(1+q^{n-1/2} y^{-1})\\
\th_4(v|\tau)= \sum (-1)^n q^{n^2/2} y^n 
&=\prod (1-q^n)(1-q^{n-1/2} y)(1-q^{n-1/2} y^{-1})
  \end{array}
\end{equation}

