\begin{equation} \label{1^6-char}
  \begin{array}{lll}
A := {\rm ch}_{0,0}^{\rm NS}(y,q) = {1\over \eta}
\theta_{0,3}({\tau\over 2}, {z\over 3}) &= {1\over \eta}
\sum_\Z q^{{3\over 2} n^2} y^n &= {1\over \eta} ~\th_3(z|3\tau) \\
B := {\rm ch}_{1,1}^{\rm NS}(y,q) = {1\over \eta} 
\theta_{2,3}({\tau\over 2}, {z\over 3}) &= {1\over \eta}
\sum_\Z q^{{3\over 2} (n+{1\over 3})^2} y^{n+{1\over 3}} &= {1\over
  \eta} q^{1/6} y^{1/3}~ \th_3(z+\tau |3\tau)\\  
C := {\rm ch}_{1,-1}^{\rm NS}(y,q) = {1\over \eta} 
\theta_{4,3}({\tau\over 2}, {z\over 3}) &= {1\over \eta}
\sum_\Z q^{{3\over 2} (n+{2\over 3})^2} y^{n+{2\over 3}} &= {1\over
  \eta} q^{2/3} y^{2/3}~\th_3(z+2\tau |3\tau) \\
&&= {1\over \eta}q^{1/6} y^{-1/3}~ \th_3(z-\tau |3\tau)
  \end{array}
\end{equation}

