\begin{equation}
  \begin{split}
    a(\tau) &= {q^{1\over 24} \over\eta} \p_y|_1 ~\sum_\Z
    (-1)^n y^{6n+1} q^{n(3n+1)/2} \\
&= {q^{1\over 24} \over\eta} \p_y|_1 ~
    y~\th_3(6z+{1+\tau\over 2}|3\tau)  \\
&= {q^{1\over 24} \over\eta} \p_y|_1 ~ y~\prod
    (1-q^{3n})(1-y^{6n}q^{3n-1})(1-y^{-6n}q^{3n-2}) \\
&= 1+ 6 \sum_{n\geq 1} \left( {-q^{3n-1} \over 1-q^{3n-1}}+
    {q^{3n-2} \over 1-q^{3n-2}} \right)\\
&= 1+6\sum q^n \Big(\sum_{d|n \atop d\equiv 1 (3)} 1 - \sum_{d|n
    \atop d\equiv 2 (3)} 1 \Big) \\
&= 1+6\sum \delta_{3,1}(n)~q^n,
  \end{split}
\end{equation}

