\begin{equation*}
  \begin{array}{rl}
\theta_m + \theta_{m+12} - \theta_{m+24} - \theta_{m+36} 
&=  \sum \delta_n ~q^{{3\over 4}(n+{m\over 12})^2} y^{n+{m\over 12}},
\qquad \delta_n :=+,+,-,- \textrm{ for } n\equiv 0,1,2,3
\textrm{ mod } 4\\
\textrm{ for }m\equiv 2 \textrm{ mod } 8: &= \sum (q ~e^{2\pi
   i})^{{3\over 4}(n+{m\over 12})^2} y^{n+{m\over 12}} \qquad\\
&= q^{({m\over 8})^2/3 + 3/16} y^{m\over 12}~{\eta_3\over\eta_6~\eta_{3/2}}
~\th_3(z +({3\over 4}+{m\over 8})\tau|3\tau)
~\th_3(z +({3\over 4}-{m\over 8})\tau|3\tau) \\
\textrm{ and for} ~m\equiv -2 \textrm{ mod } 8: &=\sum (-1)^n (q ~e^{2\pi
   i})^{{3\over 4}(n+{m\over 12})^2} y^{n+{m\over 12}} \qquad \\
&= q^{({m\over 8})^2/3 + 3/16} y^{m\over 12}~{\eta_3\over\eta_6~\eta_{3/2}}
~\th_4(z +({3\over 4}+{m\over 8})\tau|3\tau) 
~\th_4(z +({3\over 4}-{m\over 8})\tau|3\tau) 
  \end{array}
\end{equation*}

