\begin{equation}
  \begin{array}{rll}
\theta_m + \theta_{m+24} &= \sum q^{3(n+{m\over 24})^2} y^{2(n+{m\over 24})} 
   &= q^{({m\over 8})^2/3} y^{m\over 12} ~\th_3(2z+{m\tau\over 4}|6\tau) \\
\theta_m - \theta_{m+24} &= \sum (-1)^n q^{3(n+{m\over 24})^2} y^{2(n+{m\over 24})} 
   &= q^{({m\over 8})^2/3} y^{m\over 12} ~\th_4(2z+{m\tau\over 4}|6\tau) \\
\theta_m + \theta_{m+12} + \theta_{m+24} + \theta_{m+36} 
&=  \sum q^{{3\over 4}(n+{m\over 12})^2} y^{n+{m\over 12}} 
&= q^{({m\over 8})^2/3} y^{m\over 12} ~\th_3(z+{m\tau\over
  8})|{3\tau\over 2}) \\ 
\theta_m - \theta_{m+12} + \theta_{m+24} - \theta_{m+36} 
&=  \sum (-1)^n q^{{3\over 4}(n+{m\over 12})^2} y^{n+{m\over 12}} 
&= q^{({m\over 8})^2/3} y^{m\over 12} ~\th_4(z+{m\tau\over
  8})|{3\tau\over 2})\\
  \end{array}
\end{equation}

