\begin{equation}
  \begin{array}{llll}
    \th_1'(z+{1-\tau\over 2} | \tau) &= \p_z ~q^{-1/8} y^{1/2}
    ~\th_3(z) &= i\pi ~\th_1(z+{1-\tau\over 2}|\tau) + q^{-1/8} y^{1/2}
    ~\th_3'(z|\tau)   &\stackrel{z=0}{\longrightarrow} -i
    \pi q^{-1/8} ~\th_3 \\
    \th_3'(z+{1-\tau\over 2} | \tau) &= \p_z ~-i q^{-1/8} y^{1/2}
    ~\th_1(z) &= i\pi ~\th_3(z+{1-\tau\over 2}|\tau) -i q^{-1/8} y^{1/2}
    ~\th_1'(z|\tau) &\stackrel{z=0}{\longrightarrow} -
    2\pi i q^{-1/8} ~\eta^3, 
  \end{array}
\end{equation}

