\begin{equation} \label{1^6-4^3}
  \begin{array}{rll}
A+D &= 2 c_{02} ~\th_2(2z|6\tau) +(c_{00}+c_{04}) ~\th_3(2z|6\tau)
= {1\over \eta^2} \th_3(z|3\tau)^2 &= A^2{ }_{[1^6 ~{\rm theory}]} \\
B+E &= {q^{1/3} y^{2/3}\over \eta^2} \th_3 (z+\tau|3\tau)^2 &= B^2{ }_{[1^6 ~{\rm theory}]} \\
C+F &= {q^{4/3} y^{4/3}\over \eta^2} \th_3 (z+2\tau|3\tau)^2 &= C^2{ }_{[1^6 ~{\rm theory}]} \\
G &= c_{22} ~q^{1\over 12} y^{1\over 3} ~\th_3(2z+\tau|6\tau) + 
 c_{20} ~q^{1\over 12} y^{1\over 3} ~\th_2(2z+\tau|6\tau) & \\
&= {q^{1/6} y^{1/3} \over \eta^2} ~\th_3(z|3\tau)~\th_3(z+\tau|3\tau) &= AB_{[1^6 ~{\rm theory}]} \\
H &= {q^{5/6} y \over \eta^2} ~\th_3(z+\tau|3\tau)~\th_3(z+2\tau|3\tau) &= BC_{[1^6 ~{\rm theory}]} \\
I &= {q^{2/3} y^{2/3} \over \eta^2} ~\th_3(z|3\tau)~\th_3(z+2\tau|3\tau) &= AC_{[1^6 ~{\rm theory}]},
  \end{array}
\end{equation}

