\begin{equation*}
  \begin{array}{rl}
\theta_m &= \theta_{m,24}({\tau\over 2},0) = \sum
    q^{12(n+{m\over 48})^2} =q^{({m\over
        8})^2/3}~\th_3({m\tau\over 2} |24 \tau) =\theta_{-m}\\ 
\theta_m +\theta_{m+12} -\theta_{m+24} -\theta_{m+36}
    &= \sum \delta_n q^{{3\over 4}(n+{m\over 12})^2} = \sum
    \delta_n q^{{3\over 4}(n-1-{m\over 12})^2} \\
  ({\rm for }~ m=-10,-2:)  &= \sum \delta_n q^{{3\over 4}(n-{1\over 6})^2}
    = e^{-2\pi i({m\over 8})^2/3} \sum (-1)^n (-q^{1/2})^{{3\over
    2}(n-{1\over 6})^2} = {\eta^3 \over \eta_{1/2}~\eta_2},
  \end{array} 
\end{equation*} 
