\begin{equation}
\ba{ll}
F_{0\mu}=D_{0}\phi_{l}=D_{0}\phi_{r}=0\,,~~~&~~~D_{0}\phi_{p}-\textstyle{\frac{\mu}{3\sqrt{2}}}\epsilon_{pq}\phi_{q}=0\,,\\
{}&{}\\
{}[\phi_{r},\phi_{s}]-i\textstyle{\frac{\mu}{3\sqrt{2}}}\epsilon_{rst}\phi_{t}=0\,,~~~&~~~
D_{j}\phi_{r}=[\phi_{l},\phi_{r}]=[\phi_{p},\phi_{r}]=0\,,\\
{}&{}\\
F_{12}-i[\phi_{3},\phi_{4}]=0\,,~~~&~~~D_{1}\phi_{3}-D_{2}\phi_{4}=0\,,\\
{}&{}\\
D_{1}\phi_{4}+D_{2}\phi_{3}-i[\phi_{5},\phi_{6}]=0\,,~~~&~~~D_{j}\phi_{p}+iJ_{jl}\epsilon_{pq}[\phi_{l},\phi_{q}]=0\,, \ea
\end{equation}

