\begin{equation}
\left\{
\begin{aligned}
\tilde{\psi} & = \psi - \sigma' \epsilon_r,\\
\tilde E &= E + 2 \ee^{-\sigma} \epsilon ,\\
\tilde\xi &= \xi - 2 \epsilon_r',\\
 \tilde \zeta &= \zeta -
\frac{1}{2} \left[\epsilon_\theta' +\partial_\theta
\epsilon_r - \left(\displaystyle{2\over r}+\gamma'\right)
\epsilon_\theta \right],\\
 \tilde\omega &= \omega
- {2\ee^{-\gamma} \over r^2} \partial_\theta\epsilon_\theta -
\left({2\over r}+\gamma'\right)\epsilon_r,\\
\tilde B &= B -  {1\over 2} \left( \epsilon_r + \epsilon'-\sigma'
\epsilon \right),\\
\tilde C &= C - \displaystyle {1\over 2} \left( \epsilon_\theta +
\partial_\theta \epsilon \right).
\end{aligned}
\right.
\end{equation}

