\begin{equation}
  \label{eq:mode}
  \begin{array}{ll}
  \tilde\phi(x) & ={\cal U}^\dagger\phi(x){\cal U}\\
  &= {\cal U}^\+
  \left(
    {\displaystyle\sum_n} \phi^\alpha_n(x) b_n + \phi_n^{\alpha*}(x) 
b_n^\+\right){\cal U} \\
  &={ \displaystyle\sum_n} \phi^\alpha_n (x)a_n + \phi_n^{\alpha*}(x) a_n^\+ 
\\
    &= N_\alpha {\displaystyle\sum_n}
  \left(\phi^E_n(x)+\gamma{\phi_n^E}(\bar x)\right) a_n
   + \left({\phi^E_n}(x)+\gamma{\phi_n^E}(\bar x)\right)^* a_n^\+  \\
& = N_\alpha \left( \phi_0(x) + \phi_1(x) \right)
  \end{array}
\end{equation}

