\begin{equation}
  \begin{array}{rl}
A+C &= {1\over \eta} \sqrt{\th_3\over\eta} ~\th_3(0|2\tau) 
    = {\eta(2\tau)^4 \over\eta~\eta(4\tau)^2 ~\eta(\tau/2)}
    = E^2/B \\
A-C &= {1\over \eta} \sqrt{\th_3\over\eta} ~\th_4(0|2\tau) 
    = {\eta(\tau/2) \over\eta(2\tau)}= 1/E \\
B = D &=  {1\over \eta} \sqrt{\th_3\over\eta} ~\th_2(0|2\tau)  = {\eta
  ~\eta(4\tau)^2 \over \eta(\tau/2) ~\eta(2\tau)^2 } \\
E = F &= {\eta(2\tau) \over \eta(\tau/2)} = \sqrt{\half {\th_2\over\th_4}}
  \end{array}
\end{equation}

