\begin{equation}
  \begin{array}{lll}
  \th_1(\half)=\th_2 \qquad&
  \th_1(\frac{\tau}{2})=iq^{-1/8}~\th_4 \qquad &
  \th_1(\frac{1+\tau}{2})= q^{-1/8}~\th_3\\
  \th_2(\half)=0 \qquad&
  \th_2(\frac{\tau}{2})=q^{-1/8}~\th_3 \qquad &
  \th_2(\frac{1+\tau}{2})= -iq^{-1/8}~\th_4\\
  \th_3(\half)=\th_4 \qquad &
  \th_3(\frac{\tau}{2})=q^{-1/8}~\th_2 \qquad &
  \th_3(\frac{1+\tau}{2})= 0\\
  \th_4(\half)=\th_3 \qquad &
  \th_4(\frac{\tau}{2})=0 \qquad &
  \th_4(\frac{1+\tau}{2})= q^{-1/8}~\th_2\\
  \end{array}
\end{equation}

