\begin{equation} \label{2^4-char}
  \begin{array}{lll}
A := {\rm ch}_{0,0}^{\rm NS}(y,q) &= c_{00}~\theta_{0} +c_{02}~\theta_{8} 
   &= {1\over 2\eta} \sqrt{\th_3\over\eta} ~\th_3(z|2\tau)
   + {1\over 2\eta} \sqrt{\th_4\over\eta} ~\th_4(z|2\tau)\\ 
B := {\rm ch}_{2,2}^{\rm NS}(y,q) &= c_{02}~\theta_{-4} + c_{00}~\theta_{4}
   &= {1\over 2\eta} \sqrt{\th_3\over\eta} ~\th_2(z|2\tau) 
   + {1\over 2\eta} \sqrt{\th_4\over\eta} ~i ~\th_1(z|2\tau) \\ 
C := {\rm ch}_{2,0}^{\rm NS}(y,q) &= c_{02}~\theta_{0} +c_{00}~\theta_{8} 
   &= {1\over 2\eta} \sqrt{\th_3\over\eta} ~\th_3(z|2\tau)
   - {1\over 2\eta} \sqrt{\th_4\over\eta} ~\th_4(z|2\tau)\\ 
D := {\rm ch}_{2,-2}^{\rm NS}(y,q) &= c_{02}~\theta_{4}+c_{00}~\theta_{-4} 
   &= {1\over 2\eta} \sqrt{\th_3\over\eta} ~\th_2(z|2\tau) 
   - {1\over 2\eta} \sqrt{\th_4\over\eta} ~i ~\th_1(z|2\tau) \\ 
E := {\rm ch}_{1,-1}^{\rm NS}(y,q) &= c_{11}(~\theta_{-2} + \theta_{6})
   &= {\eta(2\tau)\over\eta^2} ~q^{1\over 16} y^{-{1\over
   4}} ~\th_3(z-{\tau\over 2} |2\tau)  \\ 
F := {\rm ch}_{1,1}^{\rm NS}(y,q) &= c_{11}(~\theta_{-6} +\theta_{2}) 
   &= {\eta(2\tau)\over\eta^2} ~q^{1\over 16} y^{1\over
   4} ~\th_3(z+{\tau\over 2} |2\tau) \\ 
  \end{array}
\end{equation}

