\begin{equation}
\label{e:TBA21}
\begin{split}
\u_1(\h)& = MRe^{\h}-\log{\Bigl[-\frac{e^{\h}+\sqrt{2}+e^{-\h}}
{e^{\h}-\sqrt{2}+e^{-\h}}\Bigr]}
-\sum_{k=1}^{m}\log\tanh(-\frac{\b_k}{2}-\frac{\h}{2})\\
&- \frac{1}{2\pi}\int_{-\infty}^{\infty}d\h'\frac{\log(1+e^{-\u_2(\h')})}
{\cosh(\h-\h')},\\
\u_2(\h)& = MRe^{-\h}-\log{-\frac{e^{-\h}+\sqrt{2}+e^{\h}}{e^{-\h}-\sqrt{2}+e^{\h
}}}
-\sum_{k=1}^{m}\log\tanh(\frac{\b_k}{2}-\frac{\h}{2})\\
&- \frac{1}{2\pi}\int_{-\infty}^{\infty}d\h'\frac{\log(1+e^{-\u_1(\h')})}
{\cosh(\h-\h')}+m\pi.
\end{split}
\end{equation}

