\begin{equation}
\begin{array}{lcl}
S_{F}\left( H_{4}\right)  & = & \left( -H_{4}-\alpha \,E_{1}E_{3}\,+\frac{1}{%
2}\alpha \xi \,H_{2}E_{3}^{2}\right) e^{\alpha {E}_{4}}, \\
S_{F}\left( H_{2}\right)  & = & -H_{2}e^{-\xi {E}_{2}}, \\
S_{F}\left( {E}_{4}\right)  & = & -{E}_{4}, \\
S_{F}\left( {E}_{2}\right)  & = & -{E}_{2}, \\
S_{F}\left( E_{3}\right)  & = & - E_{3}e^{\frac{1}{2}\left( \alpha {E}%
_{4}+ \xi {E}_{2}\right) }, \\
S_{F}\left( E_{-1}\right)  & = & -E_{-1}e^{\frac{1}{2}\left( \alpha {E%
}_{4} +\xi {E}_{2}\right) }, \\
S_{F}\left( E_{1}\right)  & = & \left( -E_{1}+\frac{1}{2}\xi
H_{2}E_{3}\right) e^{\frac{1}{2}\left( \alpha {E}_{4} - \xi {E}%
_{2}\right) }, \\
S_{F}\left( E_{-2}\right)  & = & -E_{-2}e^{-\xi {E}_{2}}, \\
S_{F}\left( E_{-3}\right)  & = & \left(
\begin{array}{c}
 -E_{-3}-\alpha \left( E_{-2}
-\frac{1}{4}\xi H_2 \right)E_{3} \\
+\frac{1}{2%
}\xi H_{2}\left( E_{-1}-\alpha E_{3}\right) e^{\left( \alpha {E}%
_{4}+\xi {E}_{2}\right) }
\end{array}
\right) e^{\frac{1}{2}\left( \alpha {E%
}_{4} - \xi {E}_{2}\right) }, \\
S_{F}\left( E_{-4}\right)  & = & \left(
\begin{array}{c}
-E_{-4}+\alpha E_{1}E_{-1}- \alpha E_{-3}E_{3}
-\frac{1}{2}\alpha \xi H_{2}E_{3}E_{-1}
\\
+\left( \xi ^{-1}\alpha E_{-2}-\frac{1}{4}\alpha H_{2}\right) \left(
1-e^{\left(- \xi {E}_{2}-\alpha {E}_{4}\right) }-\frac{1}{2}%
\alpha \xi E_{3}^{2}\right)
\end{array}
\right) e^{\alpha {E}_{4}}.
\end{array}
\end{equation}

