\begin{equation}
\begin{aligned}
d\mathcal{G}^{\prime }-\mathcal{G}^{\prime }\wedge \mathcal{G}^{\prime }&=%
\frac{1}{2}d(\ast d\phi ^{i})\widetilde{H}_{i}+d(e^{\frac{1}{2%
}\alpha _{i}\phi ^{i}}\ast F^{\alpha })\widetilde{E}_{\alpha }-\frac{1}{4}d%
\phi ^{j}\wedge \ast d\phi ^{i}[H_{j},\widetilde{H}_{i}]\\
\\
&-\frac{1}{2}d\phi ^{j}\wedge e^{\frac{1}{2}\alpha _{i}\phi
^{i}}\ast F^{\alpha }[H_{j},\widetilde{E}_{\alpha }]-\frac{1}{2}e^{%
\frac{1}{2}\alpha _{i}\phi ^{i}}F^{\alpha }\wedge \ast d\phi
^{j}[E_{\alpha },\widetilde{H}_{j}] \\
\\
&-e^{\frac{1}{2}\alpha _{i}\phi ^{i}}e^{\frac{1}{2}\beta
_{i}\phi ^{i}}F^{\alpha }\wedge \ast F^{\beta }[E_{\alpha },\widetilde{E}%
_{\beta }].
\end{aligned}
\end{equation}

