\begin{equation}
\begin{array}{c}
\frac{D^{2}\xi^{\mu}}{D\tau^{2}}+\frac{1}{2}\Gamma_{\sigma\gamma}^{\mu}\xi^{%
\gamma}R_{\alpha\lambda\beta}^{\sigma}\frac{dx^{\alpha}}{d\tau}%
S^{\lambda\beta}=-R_{\alpha\lambda\beta}^{\mu}\frac{dx^{\alpha}}{d\tau}%
\xi^{\lambda}\frac{dx^{\beta}}{d\tau} \\ 
\\ 
-\frac{1}{2}[R_{\alpha\lambda\beta}^{\mu}\frac{d\xi^{\alpha}}{d\tau}%
S^{\lambda\beta}+R_{\alpha\lambda\beta}^{\mu}\frac{dx^{\alpha}}{d\tau }%
S^{\lambda\beta},_{\gamma}\xi^{\gamma}+R_{\alpha\lambda\beta}^{\mu},_{\sigma
}\xi^{\sigma}\frac{dx^{\alpha}}{d\tau}S^{\lambda\beta}].
\end{array}
\label{26}
\end{equation}

