\begin{equation}
\begin{aligned}
d(e^{\frac{1}{2}\gamma _{i}\phi ^{i}}\ast F^{\gamma })&=d(e
^{-\frac{1}{2}\gamma _{i}\phi ^{i}}e^{\gamma _{i}\phi ^{i}}\ast
F^{\gamma })\\
\\
&=-\frac{1}{2}\gamma _{j}e^{-\frac{1}{2}\gamma _{i}\phi ^{i}}d\phi ^{j}\wedge e
^{\gamma _{i}\phi ^{i}}\ast F^{\gamma }\\
\\
&+\sum\limits_{\alpha -\beta =-\gamma }
e^{-\frac{1}{2}\gamma _{i}\phi ^{i}}N_{\alpha ,-\beta }F^{\alpha
}\wedge e^{\beta _{i}\phi ^{i}}\ast F^{\beta }\\
\\
&=-\frac{1}{2}\gamma _{j}e^{\frac{1}{2}\gamma _{i}\phi ^{i}}d\phi ^{j}\wedge \ast
F^{\gamma }+\sum\limits_{\alpha -\beta =-\gamma }e^{\frac{1}{2}
\alpha _{i}\phi ^{i}}e^{\frac{1}{2}\beta _{i}\phi ^{i}}N_{\alpha
,-\beta }F^{\alpha }\wedge \ast F^{\beta }.
\end{aligned}
\end{equation}

