\begin{equation}
\begin{aligned}
d\mathbf{g}_{N}\mathbf{g}_{N}^{-1}&=de^{\chi ^{m}E_{m}}e^{-\chi ^{m}E_{m}}\\
\\
&=d\chi ^{m}E_{m}+\frac{1}{2!}[\chi ^{m}E_{m},d%
\chi ^{n}E_{n}]+\frac{1}{3!}[\chi ^{m}E_{m},[\chi ^{l}E_{l},d\chi
^{n}E_{n}]]+....\\
\\
&=d\chi ^{m}E_{m}+\frac{1}{2!}\chi ^{m}d\chi
^{n}K_{mn}^{v}E_{v}+\frac{1}{3!}\chi ^{m}\chi ^{l}d\chi
^{n}K_{ln}^{v}K_{mv}^{u}E_{u}+....\\
\\
&=\overset{\rightharpoonup}{\mathbf{E
}}\:\mathbf{\Omega }\:\overset{\rightharpoonup }{d\chi }.
\end{aligned}
\end{equation}

