\begin{equation}\label{lulymo3.14}
\begin{array}{rlll}
M_1 &=&  \frac{1}{\sqrt{2}}(e_{-1} - e_1) \, , \qquad
&
 M_2 = \frac{1}{\sqrt{2}}(e_{-3} - e_3) \, ,
\cr
M_3 &=&   \frac{1}{{2}}(e_{-4} - e_2 + e_2 - e_4) \, ,
&
\cr
N_1 &=& - \frac{1}{{2}}(e_{-2} + e_4 + e_2 + e_4) \, ,
\qquad
&
N_2 =  \frac{1}{{2}}(h_{4} - h_2) \, ,
\cr
N_3 &=&  \frac{1}{\sqrt{2}}(e_{-1} + e_1) \, ,
&
\cr
{\cal P}_0 &=&  \frac{1}{{2R}}(e_{-2} + e_{-4} - e_2 - e_4) \, ,
\qquad
&
{\cal P}_1 = \frac{1}{{2R}}(h_{4} + h_{2} ) \, ,
\cr
{\cal P}_2 &=&  -\frac{1}{{2R}}(e_{-4} - e_{-2} - e_2 + e_4) \, ,
\qquad
&
{\cal P}_3 = \frac{1}{{2R}}(e_{-3} + e_{3} ) \, ,
\end{array}
\end{equation}

