\begin{equation}
\begin{split}
\langle\boldsymbol\beta, \psi_{k}\rangle=-\langle {\text Res}(\gamma_{\mu -}),{\bf Y}\psi_{k}\rangle
={\text Res}( {\bf Y}{\underline \gamma}_{\mu}(\psi_{k}))\hspace{70pt}\\
={\text Res}( {\bf Y}(\psi_{k}[J]))
=\frac{1}{\lambda^{k}}\sum_{n\geq 1}\frac{L}{(n)!} \langle{\text Res}({\tilde G}_{k}^{(n)}(p_1, \dots, p_{n})){\tilde J}_{1}, \dots ,{\tilde J}_{n} \rangle\\
=\frac{1}{\lambda^{k}}\sum_{n\geq 1}\frac{(k+1)-\frac{E}{2}}{(n)!}\langle{\text Res}({\tilde G}_{k}^{(n)}(p_1, \dots, p_{n})){\tilde J}_{1}, \dots ,{\tilde J}_{n} \rangle,\label{z.4}
\end{split}
\end{equation}

