\begin{equation}
\left\{ 
\begin{array}{c}
\left[ x^{\mu },M^{\rho \sigma }\right] =0, \\ 
\\ 
\left[ \dot{x}^{\mu },M^{\rho \sigma }\right] =\frac{q}{m}\left( x^{\rho
}F^{\mu \sigma }-x^{\sigma }F^{\mu \rho }\right) , \\ 
\\ 
\left[ L^{\mu \nu },M^{\rho \sigma }\right] =\frac{q}{m}\left( F^{\nu \sigma
}x^{\mu }x^{\rho }-F^{\mu \sigma }x^{\upsilon }x^{\rho }+F^{\rho \mu }x^{\mu
}x^{\sigma }-F^{\rho \mu }x^{\nu }x^{\sigma }\right) \\ 
=g^{\mu \rho }M^{\nu \sigma }-g^{\nu \rho }M^{\mu \sigma }+g^{\mu \sigma
}M^{\rho \nu }-g^{\nu \sigma }M^{\rho \mu }, \\ 
\\ 
\left[ M^{\mu \nu },M^{\rho \sigma }\right] =0.
\end{array}
\right.
\end{equation}

