\begin{equation}\begin{split}\label{eq7}
{\cal L}^L_{YM} &= -\frac18{\rm tr}\Big[F^L_{\mu\nu}F^L_{\mu\nu}   +
\alpha'\big(a^L_1 F^L_{\mu\lambda}F^L_{\lambda\nu}F^L_{\nu\mu}\big)\\&
+(\alpha')^2\big(a^L_3F^L_{\mu\lambda}F^L_{\nu\lambda}F^L_{\mu\rho}F^L_{\nu\rho}+a^L_4F^L_{\mu\lambda}F^L_{\nu\lambda}F^L_{\nu\rho}F^L_{\mu\rho}\\
&+a^L_5F^L_{\mu\nu}F^L_{\mu\nu}F^L_{\lambda\rho}F^L_{\lambda\rho}
+a^L_6F^L_{\mu\nu}F^L_{\lambda\rho}F^L_{\mu\nu}F^L_{\lambda\rho}\big)
+\ldots \Big]\end{split}\end{equation}

