\begin{equation}
\begin{array}{rcl}
(X^m)^{\dagger} &=& X^m,\\
\theta^{\dagger}_{\alpha} &=&
\bar{\theta}_{\dot\alpha}, \\
p_{\alpha}^{\dagger}     &=&
-\bar{p}_{\dot\alpha} ,\\
(\Gamma^{-j})^{\dagger} &=& \frac{1}{2}
\epsilon^{jkl}\Gamma^{-k}\Gamma^{-l}e^{-\rho},
\\
(\Gamma^{+j})^{\dagger}    &=& \frac{1}{2}
\epsilon^{jkl}\Gamma^{+k}\Gamma^{+l}e^{\rho}
,\\
(e^{\rho})^{\dagger} &=& \frac{1}{6}
e^{-2\rho}\epsilon^{jkl}\Gamma^{-j}\Gamma^{-k}\Gamma^{-l},
\\
(X^{-j})^{\dagger} &=& X^{-j} ,\\
(X^{+j})^{\dagger} &=& X^{+j}.
\end{array}
\end{equation}

