\begin{equation}
\begin{array}{rrl}
\cr [ E_2 , E_{-1} ]& =& - \frac{\alpha}{\xi} E_3 \, ,
\qquad \qquad \qquad\qquad\qquad \qquad
 [ E_2 , E_{-2} ] = - H_2 \, ,
\cr
 [ E_2 , E_{-3} ]& =& - ( \frac{\alpha}{2}E_3 - E_{-1})e^{\xi E_2}
+\frac{\alpha}{\xi} E_1 \, ,
\cr [ E_2 , E_{-4} ]& =&  \frac{\alpha}{\xi} H_2
    -  ( \alpha E_{-1} - \frac{1}{4} \alpha^2 E_3)\, E_3 \,
    e^{- \alpha E_4} - \frac{\alpha}{2 \xi} (e^{-\alpha E_4}
    - e^{\xi E_2}) \, ,
\cr [ E_3 , E_{-1} ]& =& \frac{1}{\xi}
    \left( e^{-\xi E_2 - \alpha E_4}-1 \right)
    + \frac{\alpha}{2} E^2_3  \, ,
\cr [ E_3 , E_{-2} ]& =& E_1
    +\xi \frac{1}{2}(\frac{1}{2}-H_2 )\, E_3 \, ,
\qquad\qquad
[ E_3 , E_{-3} ] =  \frac{1}{2} \left( H_2 + H_4 \right)\, ,
\cr [ E_3 , E_{-4} ]& =& E_{-1}e^{-\alpha E_4} -\frac{\alpha}{2}
    (H_2 + H_4)\, E_3 \, ,
\qquad\qquad [ E_4 , E_{-1} ] =  - E_3 \, ,
\cr [ E_4 , E_{-3} ]& =& E_1 \, ,
\qquad\quad\qquad\qquad \qquad\qquad\qquad \qquad [ E_4 , E_{-4} ] = H_4 \, ,
\cr [ E_{-1} ,E_{-2} ]& =& - E_{-3} - \frac{1}{2} \alpha E_1 +
    \frac{1}{2} \xi (\frac{1}{2} - H_2 )\, E_{-1} \, ,
\qquad
 [ E_{-1} , E_{-3} ] =  - E_{-4} \, ,
\cr [ E_{-1} , E_{-4} ]& =& -2\frac{\alpha}{\xi} E_{-3}
    - \frac{\alpha}{2}(H_2 + H_4)\, E_{-1} \, ,
\cr
 [ E_{-2} , E_{-3} ] &=& - \xi \frac{1}{2}(H_2 + \frac{1}{2})\, E_{-3} \, ,
\cr [ E_{-2} , E_{-4} ]& =&  \alpha E_{-3} E_1 + \frac{\alpha}{2}
    (-E_{-2} + \frac{\xi}{4}H^2_2 -\frac{1}{2}\alpha E^2_1) \, ,
\cr [ E_{-3} , E_{-4} ]& =&  \alpha H_2 \, E_{-3} - \alpha E_{-4} E_1 \, ,
\end{array}
\end{equation}

