\begin{equation}
 \begin{split}
  \partial_{\phi_{i+N}} \mathrm{tr} \left( \tilde{M}_{tN}^{n+1} \right)
  &= (n+1) \mathrm{tr} \left( \tilde{M}_{tN}^{n} \partial_{\phi_{i+N}}  \tilde{M}_{tN} \right) \\
  &= (n+1) \mathrm{tr} \left( S \tilde{M}_{tN}^{n}  S^{-1}  S ( \partial_{\phi_{i+N}}    \tilde{M}_{tN}) S^{-1} \right) \\
  &= (n+1)\mathrm{tr} \left( \tilde{M}_{tN}^{n}  ( \partial_{\phi_{i}} \tilde{M}_{tN}) \right) \\
  &= \partial_{\phi_{i}} \mathrm{tr} \left( \tilde{M}_{tN}^{n+1} \right) .
 \end{split}
\end{equation}

