\begin{equation}
\begin{array}{ccc}
  T_{abc}  & = & (D\Gamma_a)_{bc} + {1 \over 2}( \Omega_{abc} - \Omega_{acb})  \\
  T_{a{\dot 5}b} & = & (D\Gamma_a)_{{\dot5}b} + {1 \over 2}(\Omega_{a{\dot 5}b} - \Omega_{ab{\dot 5}}) \\
  T_{{\dot 5}ab} & = & (D\Gamma_{\dot 5})_{ab} + {1 \over 2}(\Omega_{{\dot 5}ab} - \Omega_{{\dot 5}ba}) \\
  T_{{\dot 5}{\dot 5}b} & = & (D\Gamma_{\dot 5})_{{\dot 5}b} +
           {1 \over 2}(\Omega_{{\dot 5}{\dot 5}b} - \Omega_{{\dot 5}b{\dot 5}}) \\
  T_{ab{\dot 5}} & = & (D\Gamma_a)_{b{\dot 5}}+
            {1 \over 2}(\Omega_{ab{\dot 5}} - \Omega_{a{\dot 5}b}) \\
  T_{{\dot 5} a {\dot 5}} & = & (D\Gamma_{{\dot 5}})_{a{\dot 5}}+
            {1 \over 2}(\Omega_{{\dot 5}a{\dot 5}} - \Omega_{{\dot 5}{\dot 5}a}) \\
  T_{a{\dot 5} {\dot 5}} & = & (D\Gamma_a)_{{\dot 5}{\dot 5}}+
            {1 \over 2}(\Omega_{a{\dot 5}{\dot 5}} + \tilde \Omega_{a{\dot 5}{\dot 5}}) \\
  T_{{\dot 5}{\dot 5}{\dot 5}} & = & (D\Gamma_{\dot 5})_{{\dot
  5}{\dot 5}} + {1 \over 2} ( \Omega_{{\dot 5}{\dot 5}{\dot 5}} + \tilde \Omega_{{\dot 5}{\dot 5}{\dot
  5}}).
\end{array}
\end{equation}

