\begin{equation}\label{llm2.11}
 \begin{array}{l}
 M_{10} = h_1 \, , \qquad M_{34} = h_3 \, ,
\qquad
  M_{02} = \frac{1}{\sqrt{2}} (e_1 +e_{-1} ) \, ,
 \cr
 M_{32} = \frac{1}{\sqrt{2}} (e_3 +e_{-3} )\, ,
 \quad
  M_{12} = -\frac{1}{\sqrt{2}} (e_1 -e_{-1} ) \, ,
  \quad
   M_{24} = \frac{1}{\sqrt{2}} (e_3 - e_{-3} )\, ,
   \cr
    M_{04} = -\frac{1}{{2}} (e_2 + e_{-2}  + e_4 + e_{-4} )\, ,
\qquad
 M_{14} = -\frac{1}{{2}} (e_2 -  e_{-2}  - e_4 + e_{-4} )\, ,
 \cr
 M_{30} = -\frac{1}{{2}} (e_2 -  e_{-2}  + e_4 - e_{-4} )\, ,
\cr
 M_{31} = -\frac{1}{{2}} (e_2 +  e_{-2}  - e_4 - e_{-4} )\, .
 \end{array}
 \end{equation}

