\begin{equation}
\begin{array}{c}
-\frac{1}{2}[R_{\alpha \lambda \beta }^{\mu }\frac{d\xi ^{\alpha }}{d\tau }%
S^{\lambda \beta }+R_{\alpha \lambda \beta }^{\mu }\frac{dx^{\alpha }}{d\tau 
}S^{\lambda \beta },_{\gamma }\xi ^{\gamma }+R_{\alpha \lambda \beta }^{\mu
},_{\sigma }\xi ^{\sigma }\frac{dx^{\alpha }}{d\tau }S^{\lambda \beta }] \\ 
\\ 
=-\frac{1}{2}[R_{\alpha \lambda \beta }^{\mu }\frac{D\xi ^{\alpha }}{D\tau }%
S^{\lambda \beta }+R_{\alpha \lambda \beta }^{\mu }\frac{dx^{\alpha }}{d\tau 
}S^{\lambda \beta };_{\gamma }\xi ^{\gamma }+R_{\alpha \lambda \beta }^{\mu
};_{\sigma }\xi ^{\sigma }\frac{dx^{\alpha }}{d\tau }S^{\lambda \beta }] \\ 
\\ 
+\frac{1}{2}\Gamma _{\sigma \gamma }^{\mu }\xi ^{\gamma }R_{\alpha \lambda
\beta }^{\sigma }\frac{dx^{\alpha }}{d\tau }S^{\lambda \beta }.
\end{array}
\label{27}
\end{equation}

