\begin{equation}
\begin{aligned}   
\frac{H^B}{\mu} =& 
       m^2 \frac{ g_{QGT}^2}{2 N_2 J}
         + 2 N^{(a)}_0 +  2 N^{(b)}_0 +
        \sum_{n \neq 0}   
              \left(1 +  \sqrt{1 + n^2\frac{g_{QGT}^2 N_2}{4 J^2}}\right)
                 \left( N^{(a)}_n  + N^{(b)}_n \right) +              \\ 
    &   +\sum_{n \neq 0} 
              \left(-1 +  \sqrt{1 + n^2\frac{g_{QGT}^2 N_2}{4 J^2}}\right) 
                  \left(\tilde{N}^{(a)}_n + \tilde{N}^{(b)}_n \right) +
       \sum_{I=5}^8 \sum_{n = -\infty}^{\infty}  \sqrt{1 + n^2 \frac{g_{QGT}^2 N_2}{4 J^2}} 
                                                                     N_n^{I},          \\ 
\frac{H^F}{\mu} =& 
        \sum_{n=-\infty}^{\infty}
        \Bigg[
           \sum_{a=1}^{2} \left(-1 + \sqrt{1 + n^2 \frac{g_{QGT}^2 N_2}{4 J^2}}\right) F^{(a)}_n +
           \sum_{a=3}^{6} \sqrt{1 + n^2 \frac{g_{QGT}^2 N_2}{4 J^2}} F^{(a)}_n +    \\ 
    &       \sum_{a=7}^{8} \left(1 + \sqrt{1 + n^2 \frac{g_{QGT}^2 N_2}{4 J^2}}\right) F^{(a)}_n
        \Bigg].
\end{aligned}
\end{equation}

