\begin{equation}
\begin{array}{c}
\frac{d^{2}\xi ^{\mu }}{d\tau ^{2}}+2\Gamma _{\alpha \beta }^{\mu }\frac{%
dx^{\alpha }}{d\tau }\frac{d\xi ^{\beta }}{d\tau }+\Gamma _{\alpha \lambda
}^{\mu },_{\beta }\frac{dx^{\alpha }}{d\tau }\frac{dx^{\beta }}{d\tau }\xi
^{\lambda }+\Gamma _{\sigma \beta }^{\mu }\Gamma _{\alpha \lambda }^{\sigma }%
\frac{dx^{\alpha }}{d\tau }\frac{dx^{\beta }}{d\tau }\xi ^{\lambda }-\Gamma
_{\sigma \lambda }^{\mu }\Gamma _{\alpha \beta }^{\sigma }\frac{dx^{\alpha }%
}{d\tau }\frac{dx^{\beta }}{d\tau }\xi ^{\lambda } \\ 
\\ 
=-R_{\alpha \lambda \beta }^{\mu }\frac{dx^{\alpha }}{d\tau }\xi ^{\lambda }%
\frac{dx^{\beta }}{d\tau }-\frac{1}{2}[R_{\alpha \lambda \beta }^{\mu }\frac{%
d\xi ^{\alpha }}{d\tau }S^{\lambda \beta }+R_{\alpha \lambda \beta }^{\mu }%
\frac{dx^{\alpha }}{d\tau }S^{\lambda \beta },_{\gamma }\xi ^{\gamma
}+R_{\alpha \lambda \beta }^{\mu },_{\sigma }\xi ^{\sigma }\frac{dx^{\alpha }%
}{d\tau }S^{\lambda \beta }],
\end{array}
\label{24}
\end{equation}

