\begin{equation}
\begin{aligned}
%%%%%%%%%%%
a_1: \qquad & (n_1,m_1)=(1,0), \qquad M_2=\frac{M_3R_2}{n_3R_1}N_2,\\
%%%%%%%%%%%%%%%%%%%%%%%%%%%%%%%%
a_2: \qquad & (N_2,M_2)=(2,0), \qquad  m_1=-\frac{M_3R_2}{n_3R_1}n_1,\\
%%%%%%%%%%%%%%%%%%%%%%%%%%%%%%%%
a_3: \qquad & (n_3,M_3)=(4^b,0), \qquad m_1=\frac{M_2}{N_2}n_1,\\
%%%%%%%%%%%%%%%%%%%%%%%%%%%%%%%%
a_4: \qquad & (n_1,m_1)=(1,1), \qquad M_2=\frac{n_3R_1+M_3R_2}{n_3R_1-M_3R_2}N_2,\\
%%%%%%%%%%%%%%%%%%%%%%%%%%%%%%%%
a_5: \qquad &(N_2,M_2)=(1,-1), \qquad  m_1=-\frac{n_3R_1+M_3R_2}{n_3R_1-M_3R_2}n_1,\\
%%%%%%%%%%%%%%%%%%%%%%%%%%%%%%%%
a_6: \qquad & (n_3,M_3)=(0,-1), \qquad m_1=-\frac{N_2}{M_2}n_1.
\end{aligned}\label{AppWrappings6SUSYcases}
\end{equation}

