\begin{equation}\label{anncoeffD}
n^{{\rm D},k}_{l_{1}L_{1}}{}^{J_{1}}\ =\ \left\{\begin{array}{ll}
N^{(k)}_{l_{1}L_{1}}{}^{J_{1}}+N^{(k)}_{(k-l_{1})L_{1}}{}^{J_{1}} &
\text{ for } J_{1},L_{1}\not= \frac{k}{2}\parbox[c][8mm][c]{0cm}{}\\
N^{(k)}_{l_{1}\frac{k}{2}}{}^{J_{1}}&
\text{ for } J_{1}\not= \frac{k}{2},\ L_{1}=[\frac{k}{2},\pm ]\parbox[c][8mm][c]{0cm}{}\\
N^{(k)}_{l_{1}L_{1}}{}^{\frac{k}{2}} &
\text{ for } J_{1}=[\frac{k}{2},\pm ],\ L_{1}\not= \frac{k}{2}\parbox[c][8mm][c]{0cm}{}\\
\delta _{l_{1}\!\!\!\mod 4}&
\text{ for } J_{1}=L_{1} = [\frac{k}{2},\pm ]\parbox[c][8mm][c]{0cm}{}\\
\delta _{l_{1}-2\!\!\! \mod 4}&
\text{ for } J_{1}= [\frac{k}{2},\pm],\ L_{1}=[\frac{k}{2},\mp]\parbox[c][8mm][c]{0cm}{}
\end{array} \right.
\end{equation}

