\begin{equation}
\begin{array}{ccc}
  \Omega_{abc}  & = & -(D\Gamma_a)_{bc} + (D\Gamma_b)_{ac} - (D\Gamma_c)_{ba} \\
  \Omega_{a{\dot 5}b} & = & - 2 (D\Gamma_a)_{{\dot 5} b} \\
  \Omega_{{\dot 5}ab} & = & 2 (D\Gamma_a)_{{\dot 5} b} \\
  T_{{\dot 5}bc} & = & (D\Gamma_{\dot 5})_{bc} + (D\Gamma_b)_{{\dot 5} c} - (D\Gamma_c)_{{\dot 5} b} \\
  T_{{\dot 5}{\dot 5}b} & = & (D\Gamma_{\dot 5})_{{\dot 5}b} \\
  T_{{\dot 5}{\dot 5}{\dot 5}} & = & (D\Gamma_{\dot 5})_{{\dot
  5}{\dot 5}}.
\end{array}
\end{equation}

