\begin{equation}
\begin{array}{c}
\frac{d^{2}(x^{\mu }+\xi ^{\mu })}{d\tau ^{2}}+(\Gamma _{\alpha \beta }^{\mu
}(x)+\Gamma _{\alpha \beta }^{\mu },_{\lambda }\xi ^{\lambda })\frac{%
d(x^{\alpha }+\xi ^{\alpha })}{d\tau }\frac{d(x^{\beta }+\xi ^{\beta })}{%
d\tau } \\ 
\\ 
=-\frac{1}{2}(R_{\alpha \lambda \beta }^{\mu }(x)+R_{\alpha \lambda \beta
}^{\mu },_{\sigma }\xi ^{\sigma })(\frac{d(x^{\alpha }+\xi ^{\alpha })}{%
d\tau })(S^{\lambda \beta }+S^{\lambda \beta },_{\gamma }\xi ^{\gamma })
\end{array}
\label{19}
\end{equation}

