\begin{equation}\label{modecond}
\begin{split}
\sum_{u=1}^3\sum_{n=1}^\infty\frac{1}{\alpha_u}(A^{(u)}CC^{-1/2}_{(u)})_{mn}(P_{n(u)C}{}^AR_{n(u)}^C
-P_{n(u)C}^{-1}{}^AR_{-n(u)}^C)\left|V_{\mbox{ferm}}\right>&=0\\
\left[\sum_{u=1}^3\sum_{n=1}^\infty(A^{(u)}C^{-1/2}_{(u)})_{mn}(P^{-1}_{n(u)C}{}^AR_{n(u)}^C
+P_{n(u)C}{}^AR_{-n(u)}^C)+B_m\Lambda^A\right]\left|V_{\mbox{ferm}}\right>&=0\\
\sum_{u=1}^3\sum_{n=1}^\infty(A^{(u)}CC^{-1/2}_{(u)})_{mn}(P^{-1}_{n(u)A}{}^CR_{n(u)C}
-P_{n(u)A}{}^CR_{-n(u)C})\left|V_{\mbox{ferm}}\right>&=0\\
\left[\sum_{u=1}^3\sum_{n=1}^\infty\alpha_u(A^{(u)}C^{-1/2}_{(u)})_{mn}(P_{n(u)A}{}^CR_{n(u)C}
+P^{-1}_{n(u)A}{}^CR_{-n(u)C})-\alpha B_m\Theta_A\right]\left|V_{\mbox{ferm}}\right>&=0\,.
\end{split}
\end{equation}

