\begin{equation}
\begin{array}{c}
\frac{D^{2}\xi ^{\mu }}{D\tau ^{2}}=-R_{\alpha \lambda \beta }^{\mu }\frac{%
dx^{\alpha }}{d\tau }\xi ^{\lambda }\frac{dx^{\beta }}{d\tau } \\ 
\\ 
-\frac{1}{2}[R_{\alpha \lambda \beta }^{\mu }\frac{D\xi ^{\alpha }}{D\tau }%
S^{\lambda \beta }+R_{\alpha \lambda \beta }^{\mu }\frac{dx^{\alpha }}{d\tau 
}S^{\lambda \beta };_{\gamma }\xi ^{\gamma }+R_{\alpha \lambda \beta }^{\mu
};_{\sigma }\xi ^{\sigma }\frac{dx^{\alpha }}{d\tau }S^{\lambda \beta }],
\end{array}
\label{28}
\end{equation}

