\begin{equation}
\left \{
\begin{array}{rcl}
x_1 &=& \displaystyle{
    \frac{m R_1}{l_s^2 p^+} \sigma +  \frac{i}{\sqrt{2 p^+}} \sum_{n = -\infty}^{\infty}
                       \left( \beta_n(\tau) e^{i n \sigma} -
                           {\beta_n(\tau)}^{\dagger} e^{-i n \sigma} \right) }\\
x_2 &=& \displaystyle{
    \frac{i}{\sqrt{2 p^+}} \sum_{n = -\infty}^{\infty}
                       \left( \gamma_n(\tau) e^{ i n \sigma} -
                           {\gamma_n(\tau)}^{\dagger} e^{- i n \sigma} \right). }\\
\end{array}
\right.
\end{equation}

